Proved CompileExprs postOk
--HG--
branch : adt

platform/cito/CompileExprs.v
@@ -13,14 +13,14 @@ Section TopLevel.
 
   Variable base dst : nat.
 
-  Definition is_state sp vs temps dst_buf : HProp :=
+  Definition is_state sp vs temps dst dst_buf : HProp :=
     (locals vars vs 0 (sp ^+ $8) *
      array temps (sp ^+ $8 ^+ $(4 * length vars)) *
      array dst_buf (sp ^+ $ dst))%Sep.
 
   Definition new_pre : assert := 
     x ~> ExX, Ex vs, Ex temps, Ex dst_buf,
-    ![^[is_state x#Sp vs temps dst_buf] * #0]x /\
+    ![^[is_state x#Sp vs temps dst dst_buf] * #0]x /\
     [| length temps = temp_size /\
        length exprs = length dst_buf |].
 
@@ -37,12 +37,12 @@ Section TopLevel.
 
   Definition runs_to x_pre x := 
     forall specs other vs temps dst_buf,
-      interp specs (![is_state x_pre#Sp vs temps dst_buf * other ] x_pre)
+      interp specs (![is_state x_pre#Sp vs temps dst dst_buf * other ] x_pre)
       -> length temps = temp_size
       -> length exprs = length dst_buf
       -> Regs x Sp = x_pre#Sp /\
       exists changed,
-        interp specs (![is_state (Regs x Sp) vs (upd_sublist temps base changed) (map (eval vs) exprs) * other ] (fst x_pre, x)) /\
+        interp specs (![is_state (Regs x Sp) vs (upd_sublist temps base changed) dst (map (eval vs) exprs) * other ] (fst x_pre, x)) /\
         length changed <= depth.
 
   Definition post (pre : assert) := 
@@ -58,11 +58,12 @@ Section TopLevel.
   Require Import SetUtil.
   Require Import Union.
 
-  Definition syn_req := 
+  Definition syn_req exprs base := 
     Subset (union_list (map free_vars exprs)) (to_set vars) /\
-    base + depth <= temp_size.
+    base + depth <= temp_size /\
+    List.Forall (fun e => DepthExpr.depth e < depth) exprs.
 
-  Definition verifCond pre := imply pre new_pre :: syn_req :: nil.
+  Definition verifCond base pre := imply pre new_pre :: syn_req exprs base :: nil.
 
   Variable imports : LabelMap.t assert.
 
@@ -103,10 +104,247 @@ Section TopLevel.
 
   Require Import Wrap.
 
+  Opaque mult.
+
   Definition compile : cmd imports modName.
-    refine (Wrap imports imports_global modName body post verifCond _ _).
+    refine (Wrap imports imports_global modName body post (verifCond base) _ _).
+
+    Lemma postOk : forall specs exprs base dst pre x,
+      interp specs (Postcondition (Seq (do_compile exprs base dst) pre) x)
+      -> imply pre (x ~> ExX, Ex vs, Ex temps, Ex dst_buf,
+        ![^[is_state x#Sp vs temps dst dst_buf] * #0]x /\
+        [| length temps = temp_size /\
+          length exprs = length dst_buf |])
+      -> syn_req exprs base
+      -> exists x0, interp specs (pre (fst x, x0))
+        /\ forall specs other vs temps dst_buf,
+          interp specs (![is_state (Regs x0 Sp) vs temps dst dst_buf * other ] (fst x, x0))
+          -> length temps = temp_size
+          -> length exprs = length dst_buf
+          -> Regs (snd x) Sp = Regs x0 Sp /\
+          exists changed,
+            interp specs (![is_state (Regs (snd x) Sp) vs (upd_sublist temps base changed) dst (map (eval vs) exprs) * other ] (fst x, snd x)) /\
+            length changed <= depth.
+      induction exprs0; post.
+
+      clear_fancy.
+      Transparent evalInstrs.
+      simpl in H3.
+      Opaque evalInstrs.
+      injection H3; clear H3; intros; subst.
+      descend.
+      eauto.
+      descend.
+      instantiate (1 := nil); simpl.
+      destruct dst_buf; simpl in *; auto.
+      discriminate.
+      simpl; auto.
+
+      apply IHexprs0 in H; clear IHexprs0; auto.
+      Focus 2.
+      hnf; post.
+      apply H0 in H3; clear H0; post.
+      unfold is_state in H2.
+      assert (interp specs0
+        (![locals vars x4 0 (Regs x2 Sp ^+ $ (8)) *
+          array x5 (Regs x2 Sp ^+ $ (8) ^+ $ (4 * Datatypes.length vars)) *
+          (array x6 (Regs x2 Sp ^+ $ (dst0)) *
+          ![fun m : ST.settings * smem => x3 m]) ] 
+        (fst x0, x2))).
+      clear H; clear_fancy.
+      step auto_ext.
+      clear H2.
+      apply H5 in H3; clear H5; post.
+      unfold stack_slot in H4.
+      clear H; clear_fancy.
+
+      Lemma array_out : forall a p,
+        length a > 0
+        -> array a p ===> p =*> Array.selN a 0 * array (tl a) (p ^+ $4).
+        clear_fancy; destruct a; unfold array; simpl; intros.
+        inversion H.
+        destruct a.
+        sepLemma.
+        apply Himp_star_frame; try apply Himp_refl.
+        eapply Himp_trans; [ apply ptsto32m_shift_base' | ].
+        instantiate (1 := 4); auto.
+        apply Himp_refl.
+      Qed.
+
+      Lemma change_hyp : forall P Q specs st,
+        interp specs (![P] st)
+        -> P ===> Q
+        -> interp specs (![Q] st).
+        intros.
+        eapply Imply_sound.
+        rewrite sepFormula_eq.
+        apply H0.
+        rewrite sepFormula_eq in *; auto.
+      Qed.
+
+      eapply change_hyp in H5.
+      Focus 2.
+      apply Himp_star_frame; [ apply Himp_refl | ].
+      apply Himp_star_frame; [ | apply Himp_refl ].
+      apply array_out; omega.
+      destruct x6; simpl in *; try discriminate.
+      evaluate auto_ext.
+      destruct x0; simpl in *.
+      descend.
+      replace (Regs x2 Sp ^+ natToW dst0 ^+ natToW 4) with (Regs x2 Sp ^+ natToW (S (S (S (S dst0)))))
+        in H9.
+      unfold is_state.
+      unfold CompileExpr.is_state in H9.
+      step auto_ext.
+      rewrite H.
+      step auto_ext.
+      rewrite <- H3.
+      step auto_ext.
+      rewrite <- wplus_assoc.
+      unfold natToW.
+      rewrite <- natToWord_plus.
+      repeat f_equal.
+      omega.
+      rewrite length_upd_sublist; auto.
+      auto.
+
+      post.
+      post.
+      eexists; split; eauto.
+      intros.
+      clear H2.
+      unfold is_state in H.
+      assert (interp specs0
+        (![CompileExpr.is_state vars (Regs x2 Sp) vs temps
+          * (array dst_buf (Regs x2 Sp ^+ $ (dst0)) * other ) ] 
+        (fst x, x2))).
+      unfold CompileExpr.is_state.
+      clear H0; clear_fancy.
+      step auto_ext.
+      clear H.
+      apply H5 in H2; clear H5.
+      generalize H6; intro Hs.
+      apply H2 in Hs; clear H2.
+      destruct x; simpl in *.
+      destruct Hs as [ ? [ ? [ ? [ ? [ ] ] ] ] ].
+      simpl in *.
+      eapply change_hyp in H2.
+      Focus 2.
+      apply Himp_star_frame; [ apply Himp_refl | ].
+      apply Himp_star_frame; [ | apply Himp_refl ].
+      apply array_out; omega.
+      unfold stack_slot in H4.
+      clear H0; clear_fancy.
+      evaluate auto_ext.
+      destruct dst_buf; simpl in *; try discriminate.
+      assert (interp specs0
+        (![is_state (Regs x0 Sp) vs (upd_sublist temps base0 x) (S (S (S (S dst0)))) dst_buf *
+          ((Regs x2 Sp ^+ natToW dst0) =*> Regs x1 Rv * other)] (s, x0))).
+      unfold is_state.
+      unfold CompileExpr.is_state in H9.
+      step auto_ext.
+      rewrite <- H0.
+      unfold natToW.
+      rewrite H.
+      rewrite <- H0.
+      step auto_ext.
+      rewrite <- wplus_assoc.
+      unfold natToW.
+      rewrite <- natToWord_plus.
+      replace (dst0 + 4) with (S (S (S (S dst0)))) by omega.
+      step auto_ext.
+      clear H9.
+      apply H3 in H10; clear H3; auto.
+      post.
+      congruence.
+
+      assert (length (upd_sublist (upd_sublist temps base0 x) base0 x3)
+        = length temps).
+      repeat rewrite length_upd_sublist; reflexivity.
+      eapply CompileExpr.get_changed in H9.
+      post.
+      descend.
+      rewrite <- H12.
+      Focus 3.
+      instantiate (1 := base0 + max (length x) (length x3)).
+      omega.
+      Focus 2.
+      destruct H1.
+      destruct (NPeano.Nat.max_spec (length x) (length x3)); intuition.
+      inversion_clear H16.
+      omega.
+      unfold is_state in *.
+      eapply change_hyp.
+      Focus 2.
+      apply Himp_star_frame; [ | eapply Himp_refl ].
+      apply Himp_star_frame; [ eapply Himp_refl | ].
+
+      Lemma array_in : forall a p,
+        length a > 0
+        -> p =*> Array.selN a 0 * array (tl a) (p ^+ $4) ===> array a p.
+        clear_fancy; destruct a; unfold array; simpl; intros.
+        inversion H.
+        destruct a.
+        sepLemma.
+        apply Himp_star_frame; try apply Himp_refl.
+        eapply Himp_trans; [ | apply ptsto32m_shift_base ].
+        instantiate (1 := 4); auto.
+        apply Himp_refl.
+        auto.
+      Qed.
+
+      apply array_in; simpl; auto.
+      simpl.
+      replace (Regs s0 Sp ^+ $ (dst0) ^+ $ (4))
+        with (Regs s0 Sp ^+ ($ (dst0) ^+ $ (4))) by words.
+      rewrite <- natToWord_plus.
+      replace (dst0 + 4) with (S (S (S (S dst0)))) by omega.
+      generalize dependent (map (eval vs) exprs0); intros.
+      step auto_ext.
+      replace (Regs x2 Sp) with (Regs s0 Sp) by congruence.
+      step auto_ext.
+
+      intros.
+      repeat rewrite CompileExpr.upd_sublist_unchanged by auto; reflexivity.
+
+      intros.
+      generalize (Max.le_max_l (length x) (length x3)).
+      generalize (Max.le_max_r (length x) (length x3)); intros.
+      repeat rewrite CompileExpr.upd_sublist_unchanged_high by auto; reflexivity.
+
+      rewrite length_upd_sublist; auto.
+      unfold syn_req in *; intuition.
+      hnf; intros.
+      apply H2.
+      simpl.
+      unfold union_list.
+      simpl.
+
+      Lemma In_union_list : forall x exprs0 acc acc',
+        In x (fold_left union (map free_vars exprs0) acc)
+        -> Subset acc acc'
+        -> In x (fold_left union (map free_vars exprs0) acc').
+        induction exprs0; simpl; intros.
+        apply H0; auto.
+        eapply IHexprs0; eauto.
+        hnf; intros.
+        apply StringFacts.union_iff.
+        apply StringFacts.union_iff in H1.
+        intuition.
+      Qed.
+
+      eapply In_union_list; eauto.
+      hnf; intros.
+      apply StringFacts.empty_iff in H5; tauto.
+      inversion H4; auto.
+    Qed.
+
+    abstract (unfold verifCond; wrap0;
+      match goal with
+        | [ H : interp _ _ |- _ ] => eapply postOk in H; post; descend; eauto
+      end).
+
     admit.
-    admit.
- Defined.
+  Defined.
 
 End TopLevel.
